Finished fault-free TMR proof

Examples/tmr/tmr_ft_proof.v
@@ -14,17 +14,36 @@ Section Invariants.
     Variable raddr : addr.
     Variable in_a in_b : addr.
     Variable len : N.
-    Variable s0 s1 s2 s3 s4 : N.
+    Variable s0 s1 s2 s3 s4 sp : N.
 
-    Definition k_equal (p1 p2 : addr) (k : N) : Prop :=
+    Definition k_equal (p1 p2 : addr) (k : N) (mem : memory) : Prop :=
         forall (i : N),
             i < k ->
             mem Ⓑ[p1 + i] = mem Ⓑ[p2 + i].
 
     (* The output of CRYPTO_memcmp is zero if and only if the two
        memory regions match up to `len` bytes *)
-    Definition postcondition (s : store) : Prop :=
-        s R_A0 = 0 <-> k_equal in_a in_b len.
+    Definition postcondition (s : store)
+            (altret : option riscvvar) 
+            (altmem : option memory): Prop :=
+        s (match altret with None => R_A0 | Some x => x end) = 0 
+            <-> 
+        k_equal in_a in_b len
+          (match altmem with None => mem | Some x => x end).
+
+    Definition ssize : N := 32.
+
+    Definition noverlaps (sp : addr) :=
+        ~ overlap 32 in_a len (sp ⊖ ssize) ssize /\
+        ~ overlap 32 in_b len (sp ⊖ ssize) ssize.
+
+    Definition stack (s : store) :=
+        s V_MEM32 = mem[Ⓓ sp ⊖ 4 :=  raddr]
+                       [Ⓓ sp ⊖ 8 :=  s0]
+                       [Ⓓ sp ⊖ 12 := s1]
+                       [Ⓓ sp ⊖ 16 := s2]
+                       [Ⓓ sp ⊖ 20 := s3]
+                       [Ⓓ sp ⊖ 24 := s4].
 
     Definition invs T (Inv Post: inv_type T) (NoInv:T) (s:store) (a:addr) : T :=
         match a with
@@ -34,7 +53,9 @@ Section Invariants.
               s V_MEM32 = mem /\
               s R_RA = raddr /\
               s R_S0 = s0 /\ s R_S1 = s1 /\ s R_S2 = s2 /\
-                s R_S3 = s3 /\ s R_S4 = s4)
+                s R_S3 = s3 /\ s R_S4 = s4 /\
+             s R_SP = sp /\
+             s V_MEM32 = mem)
         | 0x10180 => Inv 0
             (exists k,
               s V_MEM32 = mem /\
@@ -42,22 +63,49 @@ Section Invariants.
               s R_A1 = in_b ⊕ k /\
               s R_A2 = in_a ⊕ len /\
               k < len < 2^32 /\
-              ((s R_A0 = 0) <-> k_equal in_a in_b k) /\
+              ((s R_A0 = 0) <-> k_equal in_a in_b k mem) /\
               s R_RA = raddr /\
               s R_S0 = s0 /\ s R_S1 = s1 /\ s R_S2 = s2 /\
-                s R_S3 = s3 /\ s R_S4 = s4
+                s R_S3 = s3 /\ s R_S4 = s4 /\
+              s R_SP = sp /\
+              s V_MEM32 = mem
             )
         | 0x1019c | 0x101a4 => Post 0 
-            (postcondition s /\ 
+            (postcondition s None None /\ 
              s R_RA = raddr /\
              s R_S0 = s0 /\ s R_S1 = s1 /\ s R_S2 = s2 /\
-                s R_S3 = s3 /\ s R_S4 = s4)
+                s R_S3 = s3 /\ s R_S4 = s4 /\
+             s R_SP = sp /\
+             s V_MEM32 = mem)
 
         (* passwords_match_tmr *)
         | 0x101a8 => Inv 1
             (s R_A0 = in_a /\ s R_A1 = in_b /\ s R_A2 = len /\
-              s V_MEM32 = mem)
-        | 0x102b0 | 0x102b4 => Post 1 (postcondition s)
+             s R_S0 = s0 /\ s R_S1 = s1 /\ s R_S2 = s2 /\
+             s R_S3 = s3 /\ s R_S4 = s4 /\ s R_SP = sp /\
+             s R_RA = raddr /\
+              s V_MEM32 = mem /\ noverlaps (s R_SP))
+        | 0x10208 => Inv 1
+            (s R_A0 = in_a /\ s R_A1 = in_b /\ s R_A2 = len /\
+             s R_S0 = in_a /\ s R_S1 = in_b /\ s R_S2 = len /\
+             postcondition s (Some R_S3) (Some (s V_MEM32)) /\
+             noverlaps (s R_SP ⊕ ssize) /\
+             stack s)
+        | 0x1021c => Inv 1
+            (s R_A0 = in_a /\ s R_A1 = in_b /\ s R_A2 = len /\ 
+             s R_S0 = in_a /\ s R_S1 = in_b /\ s R_S2 = len /\
+             postcondition s (Some R_S4) (Some (s V_MEM32)) /\
+             postcondition s (Some R_S3) (Some (s V_MEM32)) /\
+             noverlaps (s R_SP ⊕ ssize) /\
+             stack s)
+        | 0x10220 => Inv 1
+            (postcondition s (Some R_S4) (Some (s V_MEM32)) /\
+             postcondition s (Some R_S3) (Some (s V_MEM32)) /\
+             postcondition s None (Some (s V_MEM32)) /\
+             stack s)
+        | 0x102b0 | 0x102b4 => Post 1 (
+            s R_A0 = 1 <-> k_equal in_a in_b len (s V_MEM32)
+        )
         | _ => NoInv
         end.
 
@@ -71,17 +119,17 @@ Section Invariants.
 End Invariants.
 
 Lemma k_equal_inv : forall mem a b k,
-    k_equal mem a b (1 + k) ->
-    k_equal mem a b k.
+    k_equal a b (1 + k) mem ->
+    k_equal a b k mem.
 Proof.
     intros. unfold k_equal in *.
     intros. apply H. lia.
 Qed.
 
 Lemma k_equal_step : forall mem a b k,
-    k_equal mem a b k ->
+    k_equal a b k mem ->
     mem Ⓑ[a + k] = mem Ⓑ[b + k] ->
-    k_equal mem a b (1 + k).
+    k_equal a b (1 + k) mem.
 Proof.
     intros. unfold k_equal in *.
     intros. assert (i = k \/ i < k) by lia. destruct H2.
@@ -102,7 +150,7 @@ Qed.
 
 (* Proof in fault-free context *)
 Theorem crypto_memcmp_correctness:
-  forall s mem t xs' in_a in_b len raddr s0 s1 s2 s3 s4
+  forall s mem t xs' in_a in_b len raddr s0 s1 s2 s3 s4 sp
          (ENTRY: startof t xs' = (Addr 0x10170, s))
          (MDL: models rvtypctx s)
          (MEM: s V_MEM32 = mem)
@@ -114,9 +162,11 @@ Theorem crypto_memcmp_correctness:
          (S1: s R_S1 = s1)
          (S2: s R_S2 = s2)
          (S3: s R_S3 = s3)
-         (S4: s R_S4 = s4),
-  satisfies_all tmr_ft (invs0 mem raddr in_a in_b len s0 s1 s2 s3 s4)
-                       (exits0 mem raddr in_a in_b len s0 s1 s2 s3 s4) (xs'::t).
+         (S4: s R_S4 = s4)
+         (SP: s R_SP = sp),
+  satisfies_all tmr_ft (invs0 mem raddr in_a in_b len s0 s1 s2 s3 s4 sp)
+                       (exits0 mem raddr in_a in_b len s0 s1 s2 s3 s4 sp)
+                       (xs'::t).
 Proof using.
     Local Ltac step := time r5_step.
     intros. apply prove_invs.
@@ -176,7 +226,7 @@ Qed.
 
 (* Proof in fault-free environment *)
 Theorem tmr_ft_correctness:
-  forall s mem t xs' in_a in_b len raddr s0 s1 s2 s3 s4
+  forall s mem t xs' in_a in_b len raddr s0 s1 s2 s3 s4 sp
          (ENTRY: startof t xs' = (Addr 0x101a8, s))
          (MDL: models rvtypctx s)
          (MEM: s V_MEM32 = mem)
@@ -188,24 +238,24 @@ Theorem tmr_ft_correctness:
          (S1: s R_S1 = s1)
          (S2: s R_S2 = s2)
          (S3: s R_S3 = s3)
-         (S4: s R_S4 = s4),
-  satisfies_all tmr_ft (invs1 mem raddr in_a in_b len s0 s1 s2 s3 s4)
-                       (exits1 mem raddr in_a in_b len s0 s1 s2 s3 s4) (xs'::t).
+         (S4: s R_S4 = s4)
+         (SP: s R_SP = sp)
+         (NVL: noverlaps in_a in_b len sp),
+  satisfies_all tmr_ft (invs1 mem raddr in_a in_b len s0 s1 s2 s3 s4 sp)
+                       (exits1 mem raddr in_a in_b len s0 s1 s2 s3 s4 sp) (xs'::t).
 Proof.
     intros. apply prove_invs.
 
-    simpl. rewrite ENTRY. step. repeat split; assumption.
+    simpl. rewrite ENTRY. step. rewrite SP.
+    repeat (split; auto).
 
     intros.
     eapply startof_prefix in ENTRY; try eassumption.
     eapply preservation_exec_prog in MDL; try (eassumption || apply lift_riscv_welltyped).
-    clear - PRE MDL. rename t1 into t. rename s1 into s. rename a1 into a.
+    clear - PRE MDL. rename t1 into t. rename s5 into s. rename a1 into a.
 
     destruct_inv 32 PRE.
 
-    (* Intro *)
-    destruct PRE as (A0 & A1 & A2 & Mem).
-    do 20 step.
     Ltac riscv_call thm :=
         let MDL1 := fresh "MDL1" in
         let s1 := fresh "s1" in
@@ -213,7 +263,9 @@ Proof.
         eapply models_after_steps;
         [assumption|apply lift_riscv_welltyped|];
         intro MDL1; eapply (perform_call 0);
-        [reflexivity|eauto using thm|reflexivity|];
+        [reflexivity|intros;
+                     eapply thm; 
+                     try reflexivity; eauto|reflexivity|];
         let a := fresh "a" in
         let s' := fresh "s'" in
         let t2 := fresh "t2" in
@@ -224,163 +276,237 @@ Proof.
         assert (models rvtypctx s') as MDL' by
             (eapply preservation_exec_prog;
              eauto using lift_riscv_welltyped);
+        unfold archtyps in *;
         match goal with
         | [|- context[?t2 ++ ?t0 ++ (Addr ?x, ?s) :: ?t]] =>
             let t' := fresh "t'" in
             set (t' := t2++t0++(Addr x, s)::t) in *; clearbody s1;
-            (* repeat match goal with
-            | [PRE: true_inv _ |- _] =>
-                let x := fresh "x" in
-                set (x := s _) in PRE; clearbody x
-            end *)
-            clear - PRE MDL';
             let MDL := fresh "MDL" in
             rename MDL' into MDL;
             destruct_inv 32 PRE
         end.
-    (* Call CRYPTO_memcmp *)
-    riscv_call crypto_memcmp_correctness.
-
-    - destruct PRE as (Answer1 & RA & S0 & S1 & S2 & S3 & S4).
-      unfold postcondition in Answer1.
-      destruct (N.eq_dec (s' R_A0) 0).
-      -- (* A0 = 0 *)
-        apply Answer1 in e.
-        do 6 step. riscv_call crypto_memcmp_correctness.
-        destruct PRE as (Answer2 & RA & S0 & S1 & S2 & S3 & S4).
-      -- (* A0 <> 0 *)
-        
-         do 6 step;
-         riscv_call crypto_memcmp_correctness.
-
-Section FaultTolerantInvariants.
-    Variable mem : memory.
-    Variable in_a in_b : addr.
-    Variable len : N.
-
-    Definition ft_invs T (Inv Post: inv_type T) (NoInv:T) (s:store) (a:addr) : T :=
-        match a with
-        | 0x0 => Inv 0
-            (s R_A0 = in_a /\ s R_A1 = in_b /\ s R_A2 = len /\
-              s V_MEM32 = mem /\ s V_FC = 1)
-        | 0x28 => Inv 0
-            (exists k,
-              s V_MEM32 = mem /\
-              s R_A5 = in_a ⊕ k /\
-              s R_A1 = in_b ⊕ k /\
-              s R_A2 = in_a ⊕ len /\
-              k < len < 2^32 /\
-              s V_FC <= 1 /\
-              ((s R_A0 = 0) <-> k_equal mem in_a in_b k)
-            )
-        | 0x80 | 0x84 | 0x90 | 0x94 => Post 0 (postcondition mem in_a in_b len s)
-        | _ => NoInv
-        end.
-
-    Definition fault_memcmp := inject_fault memcmp.
-
-    Definition ft_exits0 := make_exits 0 fault_memcmp ft_invs.
-    Definition ft_invs0 := make_invs 0 fault_memcmp ft_invs.
-End FaultTolerantInvariants.
-    
-(* Proof in fault-free context *)
-Theorem crypto_memcmp_ft_correctness:
-  forall s mem t xs' in_a in_b len
-         (ENTRY: startof t xs' = (Addr 0, s))
-         (MDL: models rvtypctx s)
-         (MEM: s V_MEM32 = mem)
-         (A0: s R_A0 = in_a)
-         (A1: s R_A1 = in_b)
-         (LEN: s R_A2 = len)
-         (FC: s V_FC = 1),
-  satisfies_all fault_memcmp
-                       (ft_invs0 mem in_a in_b len)
-                       (ft_exits0 mem in_a in_b len) (xs'::t).
-Proof using.
-    Local Ltac step ::= 
-        match goal with
-        | [s' : store, FC : ?s' V_FC <= 1 |- _] =>
-            let H := fresh "H" in
-            assert (s' V_FC = 0 \/ s' V_FC = 1) as H by lia;
-            clear FC; destruct H
-        | _ => idtac
-        end;
-        time r5_step;
-        repeat match goal with
-        | [n : N, BC : ?n mod 2 = _ |- _] => clear BC n
-        | [s' : store, n : N, 
-            BC : (if 0 <? ?s' V_FC then ?n mod 2 else 0) = _ |- _] => clear BC n
-        | [H: ?x = ?x |- _] => clear H
-        end;
-        try discriminate.
-    intros. apply prove_invs.
-
-    simpl. rewrite ENTRY. step. repeat split; assumption.
-
-    intros.
-    eapply startof_prefix in ENTRY; try eassumption.
-    eapply preservation_exec_prog in MDL; try (eassumption || apply inject_fault_lift_riscv_welltyped).
-    clear - PRE MDL. rename t1 into t. rename s1 into s. rename a1 into a.
-
-    destruct_inv 32 PRE.
 
     (* Intro *)
-    destruct PRE as (A0 & A1 & A2 & Mem & FC). {
-    Local Ltac solve_inv MDL A2 :=
-        exists 0; psimpl; repeat split; auto;
-            [lia|
-            apply (models_var R_A2) in MDL; rewrite <- A2; apply MDL
-            |lia|unfold k_equal; lia].
-    step.
-    - (* len = 0, no fault *)
-        repeat step; split; intro;
-            unfold k_equal; lia.
-    - (* len <> 0, no fault *)
-        repeat (step; [| repeat step; solve_inv MDL A2]); solve_inv MDL A2.
-    - (* fault *) 
-        repeat step.
-            split; intro; unfold k_equal; lia.
-        solve_inv MDL A2.
+    destruct PRE as (A0 & A1 & A2 & S0 & S1 & S2 & S3 & S4 & SP & RA & Mem & NVL). {
+    do 20 step.
+
+    (* Dummy hyp to make it easier to use the above tactic *)
+    eassert (ST: stack mem raddr s0 s1 s2 s3 s4 sp 
+        (update s V_MEM32 _)).
+        unfold stack; now psimpl.
+
+    (* Call CRYPTO_memcmp *)
+    riscv_call crypto_memcmp_correctness;
+        (destruct PRE as (Answer1 & RA' & S0' & S1' & S2' & S3' & S4' & SP' & Mem');
+        unfold postcondition in Answer1; repeat step;
+        repeat (split; [reflexivity|]); split; [
+            unfold postcondition; split; intro; [
+                apply Answer1 in H; intros a ALen;
+                specialize (H a ALen);
+                repeat (rewrite getmem_noverlap in H; [|
+                    ((apply (noverlap_shrink _ in_a len);
+                        [psimpl; lia|]) ||
+                    (apply (noverlap_shrink _ in_b len);
+                        [psimpl; lia|]));
+                    apply noverlap_symmetry,
+                        (noverlap_shrink _ (s5 R_SP ⊖ 32) 32);
+                        [psimpl; lia|];
+                    apply noverlap_symmetry; now destruct NVL]);
+                rewrite Mem';
+                now repeat (rewrite getmem_noverlap; [|
+                    ((apply (noverlap_shrink _ in_a len);
+                        [psimpl; lia|]) ||
+                    (apply (noverlap_shrink _ in_b len);
+                        [psimpl; lia|]));
+                    apply noverlap_symmetry,
+                        (noverlap_shrink _ (s5 R_SP ⊖ 32) 32);
+                        [psimpl; lia|];
+                    apply noverlap_symmetry; now destruct NVL])
+            | psimpl; apply Answer1; intros a ALen;
+                specialize (H a ALen);
+                rewrite Mem' in H;
+                repeat (rewrite getmem_noverlap in H; [|
+                    ((apply (noverlap_shrink _ in_a len);
+                        [psimpl; lia|]) ||
+                    (apply (noverlap_shrink _ in_b len);
+                        [psimpl; lia|]));
+                    apply noverlap_symmetry,
+                        (noverlap_shrink _ (s5 R_SP ⊖ 32) 32);
+                        [psimpl; lia|];
+                    apply noverlap_symmetry; now destruct NVL
+                ]);
+                now repeat (rewrite getmem_noverlap; [|
+                    ((apply (noverlap_shrink _ in_a len);
+                        [psimpl; lia|]) ||
+                    (apply (noverlap_shrink _ in_b len);
+                        [psimpl; lia|]));
+                    apply noverlap_symmetry,
+                        (noverlap_shrink _ (s5 R_SP ⊖ 32) 32);
+                        [psimpl; lia|];
+                    apply noverlap_symmetry; now destruct NVL])]
+        |]; split; [unfold noverlaps in *; psimpl; 
+            now rewrite SP', <- SP
+        |unfold stack; psimpl; now rewrite Mem']).
     }
 
-    (* Loop *)
-    destruct PRE as (k & Mem & A5 & A1 & A2 & Bound & FC & Eq). {
-    Local Ltac solve_inv' k Eq :=
-        let X := fresh "X" in
-        let Y := fresh "Y" in
-        let Z := fresh "Z" in
-        let W := fresh "W" in
-        let Inv := fresh "Inv" in
-        let i := fresh "i" in
-        exists (k ⊕ 1); psimpl; repeat split;
-        [lia|lia|lia
-        | unfold k_equal; intros X i Z; apply or_xor_zero in X; destruct X;
-            assert (i < k \/ i = k) as Y by lia; destruct Y;
-            [now apply Eq|now subst]
-        | repeat split; intros W; rewrite N.mod_small in W by lia;
-            pose proof (k_equal_inv _ _ _ _ W) as Inv; apply Eq in Inv;
-            specialize (W k ltac:(lia));
-            now rewrite W, N.lxor_nilpotent, Inv].
-    Local Ltac solve_post k len s Eq :=
-        let X := fresh "H" in
-        let i := fresh "i" in
-        let ILen := fresh "ilen" in
-        let KLen := fresh "klen" in
-        assert (1 + k = len) as KLen by lia;
-        subst len;
-        split; intro X;
-            [apply k_equal_step;
-              apply or_xor_zero in X; destruct X;
-              [apply Eq; assumption|now symmetry]
-            |replace (s R_A0) with 0; psimpl;
-              [apply N.lxor_eq_0_iff; symmetry; apply X; lia
-              |apply k_equal_inv in X; symmetry; apply Eq, X]
-            ].
-    repeat step.
-    par: match goal with
-        | [ |- context[exists _, _] ] => solve_inv' k Eq
-        | [ |- context[_ /\ _]] => solve_post k len s Eq
-        | _ => idtac
-        end.
+    (* To second call *)
+    destruct PRE as (A0 & A1 & A2 & S0 & S1 & S2 & Answer1 & NVL & ST). {
+    step.
+
+    (* Formal goal for riscv_call*)
+    match goal with
+    | [|- context[?x :: ?y :: ?t]] =>
+        change (x :: y :: t) with
+            (x :: nil ++ y :: t)
+    end.
+
+    (* Call CRYPTO_memcmp *)
+    riscv_call crypto_memcmp_correctness;
+        (destruct PRE as (Answer2 & RA & S0' & S1' & S2' & S3 & S4 & SP & MEM);
+        unfold postcondition in Answer2; repeat step;
+        repeat (split; [solve[reflexivity||auto]|]); split; [
+            unfold postcondition; split; intro; [
+                apply Answer2 in H; intros a ALen;
+                rewrite A2 in H;
+                specialize (H a ALen);
+                repeat (rewrite getmem_noverlap in H; [|
+                    ((apply (noverlap_shrink _ in_a len);
+                        [psimpl; lia|]) ||
+                    (apply (noverlap_shrink _ in_b len);
+                        [psimpl; lia|]));
+                    apply noverlap_symmetry,
+                        (noverlap_shrink _ (s5 R_SP ⊖ 32) 32);
+                        [psimpl; lia|];
+                    apply noverlap_symmetry; now destruct NVL]);
+                rewrite MEM;
+                rewrite A0, A1 in H;
+                now repeat (rewrite getmem_noverlap; [|
+                    ((apply (noverlap_shrink _ in_a len);
+                        [psimpl; lia|]) ||
+                    (apply (noverlap_shrink _ in_b len);
+                        [psimpl; lia|]));
+                    apply noverlap_symmetry,
+                        (noverlap_shrink _ (s5 R_SP ⊖ 32) 32);
+                        [psimpl; lia|];
+                    apply noverlap_symmetry; now destruct NVL])
+            | psimpl; apply Answer2; intros a ALen;
+                rewrite A2 in ALen;
+                specialize (H a ALen);
+                rewrite MEM in H;
+                repeat (rewrite getmem_noverlap in H; [|
+                    ((apply (noverlap_shrink _ in_a len);
+                        [psimpl; lia|]) ||
+                    (apply (noverlap_shrink _ in_b len);
+                        [psimpl; lia|]));
+                    apply noverlap_symmetry,
+                        (noverlap_shrink _ (s5 R_SP ⊖ 32) 32);
+                        [psimpl; lia|];
+                    apply noverlap_symmetry; now destruct NVL
+                ]);
+                rewrite A0, A1;
+                now repeat (rewrite getmem_noverlap; [|
+                    ((apply (noverlap_shrink _ in_a len);
+                        [psimpl; lia|]) ||
+                    (apply (noverlap_shrink _ in_b len);
+                        [psimpl; lia|]));
+                    apply noverlap_symmetry,
+                        (noverlap_shrink _ (s5 R_SP ⊖ 32) 32);
+                        [psimpl; lia|];
+                    apply noverlap_symmetry; now destruct NVL])]
+        |]; split; [
+          unfold postcondition;
+          psimpl; rewrite S3, MEM; apply Answer1
+        |]; split; [unfold noverlaps in *; psimpl; 
+          psimpl in NVL; now rewrite SP|];
+          unfold stack; psimpl; rewrite MEM; apply ST).
     }
+
+    (* To third call *)
+    destruct PRE as (A0 & A1 & A2 & S0 & S1 & S2 & Answer1 & Answer2 & NVL & ST). {
+    step.
+
+    match goal with
+    | [|- context[?x :: ?y :: ?t]] =>
+        change (x :: y :: t) with
+            (x :: nil ++ y :: t)
+    end.
+
+    (* Call CRYPTO_memcmp *)
+    riscv_call crypto_memcmp_correctness;
+        (destruct PRE as (Answer3 & RA & S0' & S1' & S2' & S3 & S4 & SP & MEM);
+        repeat step; unfold postcondition in *; psimpl; split;
+        [rewrite S4, MEM; apply Answer1|]; split;
+        [rewrite S3, MEM; apply Answer2|]; split; [
+            split; intro; [
+                apply Answer3 in H; intros a ALen;
+                rewrite A2 in H;
+                specialize (H a ALen);
+                repeat (rewrite getmem_noverlap in H; [|
+                    ((apply (noverlap_shrink _ in_a len);
+                        [psimpl; lia|]) ||
+                    (apply (noverlap_shrink _ in_b len);
+                        [psimpl; lia|]));
+                    apply noverlap_symmetry,
+                        (noverlap_shrink _ (s5 R_SP ⊖ 32) 32);
+                        [psimpl; lia|];
+                    apply noverlap_symmetry; now destruct NVL]);
+                rewrite MEM;
+                rewrite A0, A1 in H;
+                now repeat (rewrite getmem_noverlap; [|
+                    ((apply (noverlap_shrink _ in_a len);
+                        [psimpl; lia|]) ||
+                    (apply (noverlap_shrink _ in_b len);
+                        [psimpl; lia|]));
+                    apply noverlap_symmetry,
+                        (noverlap_shrink _ (s5 R_SP ⊖ 32) 32);
+                        [psimpl; lia|];
+                    apply noverlap_symmetry; now destruct NVL])
+            | psimpl; apply Answer3; intros a ALen;
+                rewrite A2 in ALen;
+                specialize (H a ALen);
+                rewrite MEM in H;
+                repeat (rewrite getmem_noverlap in H; [|
+                    ((apply (noverlap_shrink _ in_a len);
+                        [psimpl; lia|]) ||
+                    (apply (noverlap_shrink _ in_b len);
+                        [psimpl; lia|]));
+                    apply noverlap_symmetry,
+                        (noverlap_shrink _ (s5 R_SP ⊖ 32) 32);
+                        [psimpl; lia|];
+                    apply noverlap_symmetry; now destruct NVL
+                ]);
+                rewrite A0, A1;
+                now repeat (rewrite getmem_noverlap; [|
+                    ((apply (noverlap_shrink _ in_a len);
+                        [psimpl; lia|]) ||
+                    (apply (noverlap_shrink _ in_b len);
+                        [psimpl; lia|]));
+                    apply noverlap_symmetry,
+                        (noverlap_shrink _ (s5 R_SP ⊖ 32) 32);
+                        [psimpl; lia|];
+                    apply noverlap_symmetry; now destruct NVL])]
+        |]; unfold stack; psimpl; rewrite MEM; apply ST).
+    }
+
+    (* Postcondition *)
+    destruct PRE as (Answer1 & Answer2 & Answer3 & ST).
+    repeat step. unfold stack in ST. split; intro.
+    - unfold postcondition in *.
+      destruct (N.eq_dec (s R_S4) 0),
+               (N.eq_dec (s R_S3) 0),
+               (N.eq_dec (s R_A0) 0);
+        ((now apply Answer1) || (now apply Answer2) || (now apply Answer3) || idtac).
+      repeat (let E := fresh "E" in
+              destruct (N.ltb 0 _) eqn:E in H; [|lia]).
+      psimpl in H. discriminate.
+    - unfold postcondition in *.
+      destruct (N.eq_dec (s R_S4) 0),
+               (N.eq_dec (s R_S3) 0),
+               (N.eq_dec (s R_A0) 0);
+        try rewrite e; try rewrite e0; try rewrite e1; psimpl;
+        auto.
+      apply Answer2 in H. contradiction.
+      apply Answer1 in H. contradiction.
+      apply Answer2 in H. contradiction.
+      apply Answer1 in H. contradiction.
 Qed.
